heap_lang/lang.v
@@ -100,6 +100,7 @@ Inductive expr :=
   | Fork (e : expr)
   (* Heap *)
   | AllocN (e1 e2 : expr) (* array length (positive number), initial value *)
+  | Free (e : expr)
   | Load (e : expr)
   | Store (e1 : expr) (e2 : expr)
   | CmpXchg (e0 : expr) (e1 : expr) (e2 : expr) (* Compare-exchange *)
@@ -186,7 +187,7 @@ Arguments vals_compare_safe !_ !_ /.
 
 (** The state: heaps of vals. *)
 Record state : Type := {
-  heap: gmap loc val;
+  heap: gmap loc (option val);
   used_proph_id: gset proph_id;
 }.
 
@@ -232,6 +233,7 @@ Proof.
      | Fork e, Fork e' => cast_if (decide (e = e'))
      | AllocN e1 e2, AllocN e1' e2' =>
         cast_if_and (decide (e1 = e1')) (decide (e2 = e2'))
+     | Free e1, Free e2 => cast_if (decide (e1 = e2))
      | Load e, Load e' => cast_if (decide (e = e'))
      | Store e1 e2, Store e1' e2' =>
         cast_if_and (decide (e1 = e1')) (decide (e2 = e2'))
@@ -318,6 +320,7 @@ Proof.
      | CmpXchg e0 e1 e2 => GenNode 16 [go e0; go e1; go e2]
      | FAA e1 e2 => GenNode 17 [go e1; go e2]
      | ChooseNat => GenNode 18 []
+     | Free e => GenNode 19 [go e]
      end
    with gov v :=
      match v with
@@ -352,6 +355,7 @@ Proof.
      | GenNode 16 [e0; e1; e2] => CmpXchg (go e0) (go e1) (go e2)
      | GenNode 17 [e1; e2] => FAA (go e1) (go e2)
      | GenNode 18 [] => ChooseNat
+     | GenNode 19 [e] => Free (go e)
      | _ => Val $ LitV LitUnit (* dummy *)
      end
    with gov v :=
@@ -366,7 +370,7 @@ Proof.
    for go).
  refine (inj_countable' enc dec _).
  refine (fix go (e : expr) {struct e} := _ with gov (v : val) {struct v} := _ for go).
- - destruct e as [v| | | | | | | | | | | | | | | | | | |]; simpl; f_equal;
+ - destruct e as [v| | | | | | | | | | | | | | | | | | | |]; simpl; f_equal;
      [exact (gov v)|done..].
  - destruct v; by f_equal.
 Qed.
@@ -401,6 +405,7 @@ Inductive ectx_item :=
   | AllocNLCtx (v2 : val)
   | AllocNRCtx (e1 : expr)
   | LoadCtx
+  | FreeCtx
   | StoreLCtx (v2 : val)
   | StoreRCtx (e1 : expr)
   | CmpXchgLCtx (v1 : val) (v2 : val)
@@ -433,6 +438,7 @@ Definition fill_item (Ki : ectx_item) (e : expr) : expr :=
   | CaseCtx e1 e2 => Case e e1 e2
   | AllocNLCtx v2 => AllocN e (Val v2)
   | AllocNRCtx e1 => AllocN e1 e
+  | FreeCtx => Free e
   | LoadCtx => Load e
   | StoreLCtx v2 => Store e (Val v2)
   | StoreRCtx e1 => Store e1 e
@@ -462,6 +468,7 @@ Fixpoint subst (x : string) (v : val) (e : expr)  : expr :=
   | Case e0 e1 e2 => Case (subst x v e0) (subst x v e1) (subst x v e2)
   | Fork e => Fork (subst x v e)
   | AllocN e1 e2 => AllocN (subst x v e1) (subst x v e2)
+  | Free e => Free (subst x v e)
   | Load e => Load (subst x v e)
   | Store e1 e2 => Store (subst x v e1) (subst x v e2)
   | CmpXchg e0 e1 e2 => CmpXchg (subst x v e0) (subst x v e1) (subst x v e2)
@@ -526,7 +533,7 @@ Definition bin_op_eval (op : bin_op) (v1 v2 : val) : option val :=
     | _, _, _ => None
     end.
 
-Definition state_upd_heap (f: gmap loc val → gmap loc val) (σ: state) : state :=
+Definition state_upd_heap (f: gmap loc (option val) → gmap loc (option val)) (σ: state) : state :=
   {| heap := f σ.(heap); used_proph_id := σ.(used_proph_id) |}.
 Arguments state_upd_heap _ !_ /.
 
@@ -534,26 +541,26 @@ Definition state_upd_used_proph_id (f: gset proph_id → gset proph_id) (σ: sta
   {| heap := σ.(heap); used_proph_id := f σ.(used_proph_id) |}.
 Arguments state_upd_used_proph_id _ !_ /.
 
-Fixpoint heap_array (l : loc) (vs : list val) : gmap loc val :=
+Fixpoint heap_array (l : loc) (vs : list val) : gmap loc (option val) :=
   match vs with
   | [] => ∅
-  | v :: vs' => {[l := v]} ∪ heap_array (l +ₗ 1) vs'
+  | v :: vs' => {[l := Some v]} ∪ heap_array (l +ₗ 1) vs'
   end.
 
-Lemma heap_array_singleton l v : heap_array l [v] = {[l := v]}.
+Lemma heap_array_singleton l v : heap_array l [v] = {[l := Some v]}.
 Proof. by rewrite /heap_array right_id. Qed.
 
-Lemma heap_array_lookup l vs w k :
-  heap_array l vs !! k = Some w ↔
-  ∃ j, 0 ≤ j ∧ k = l +ₗ j ∧ vs !! (Z.to_nat j) = Some w.
+Lemma heap_array_lookup l vs ow k :
+  heap_array l vs !! k = Some ow ↔
+  ∃ j w, 0 ≤ j ∧ k = l +ₗ j ∧ ow = Some w /\ vs !! (Z.to_nat j) = Some w.
 Proof.
   revert k l; induction vs as [|v' vs IH]=> l' l /=.
   { rewrite lookup_empty. naive_solver lia. }
   rewrite -insert_union_singleton_l lookup_insert_Some IH. split.
-  - intros [[-> ->] | (Hl & j & ? & -> & ?)].
+  - intros [[-> ?] | (Hl & j & w & ? & -> & -> & ?)].
     { exists 0. rewrite loc_add_0. naive_solver lia. }
-    exists (1 + j). rewrite loc_add_assoc !Z.add_1_l Z2Nat.inj_succ; auto with lia.
-  - intros (j & ? & -> & Hil). destruct (decide (j = 0)); simplify_eq/=.
+    eexists (1 + j)%Z, _. rewrite loc_add_assoc !Z.add_1_l Z2Nat.inj_succ; auto with lia.
+  - intros (j & w & ? & -> & -> & Hil). destruct (decide (j = 0)); simplify_eq/=.
     { rewrite loc_add_0; eauto. }
     right. split.
     { rewrite -{1}(loc_add_0 l). intros ?%(inj _); lia. }
@@ -561,15 +568,15 @@ Proof.
     { rewrite -Z2Nat.inj_succ; last lia. f_equal; lia. }
     rewrite Hj /= in Hil.
     exists (j - 1). rewrite loc_add_assoc Z.add_sub_assoc Z.add_simpl_l.
-    auto with lia.
+    eexists. split; eauto. lia. 
 Qed.
 
-Lemma heap_array_map_disjoint (h : gmap loc val) (l : loc) (vs : list val) :
+Lemma heap_array_map_disjoint (h : gmap loc (option val)) (l : loc) (vs : list val) :
   (∀ i, (0 ≤ i) → (i < length vs) → h !! (l +ₗ i) = None) →
   (heap_array l vs) ##ₘ h.
 Proof.
-  intros Hdisj. apply map_disjoint_spec=> l' v1 v2.
-  intros (j&?&->&Hj%lookup_lt_Some%inj_lt)%heap_array_lookup.
+  intros Hdisj. apply map_disjoint_spec=> l' v1 v2.  
+  intros (j&w&?&->&?&Hj%lookup_lt_Some%inj_lt)%heap_array_lookup.
   move: Hj. rewrite Z2Nat.id // => ?. by rewrite Hdisj.
 Qed.
 
@@ -578,7 +585,7 @@ Definition state_init_heap (l : loc) (n : Z) (v : val) (σ : state) : state :=
   state_upd_heap (λ h, heap_array l (replicate (Z.to_nat n) v) ∪ h) σ.
 
 Lemma state_init_heap_singleton l v σ :
-  state_init_heap l 1 v σ = state_upd_heap <[l:=v]> σ.
+  state_init_heap l 1 v σ = state_upd_heap <[l:=Some v]> σ.
 Proof.
   destruct σ as [h p]. rewrite /state_init_heap /=. f_equiv.
   rewrite right_id insert_union_singleton_l. done.
@@ -622,26 +629,31 @@ Inductive head_step : expr → state → expr → state → list expr → Prop :
      head_step (AllocN (Val $ LitV $ LitInt n) (Val v)) σ
                (Val $ LitV $ LitLoc l) (state_init_heap l n v σ)
                []
+  | FreeS l v σ :
+     σ.(heap) !! l = Some $ Some v →
+     head_step (Free (Val $ LitV $ LitLoc l)) σ
+               (Val $ LitV LitUnit) (state_upd_heap <[l:=None]> σ)
+               []
   | LoadS l v σ :
-     σ.(heap) !! l = Some v →
+     σ.(heap) !! l = Some $ Some v →
      head_step (Load (Val $ LitV $ LitLoc l)) σ (of_val v) σ []
-  | StoreS l v σ :
-     is_Some (σ.(heap) !! l) →
-     head_step (Store (Val $ LitV $ LitLoc l) (Val v)) σ
-               (Val $ LitV LitUnit) (state_upd_heap <[l:=v]> σ)
+  | StoreS l v w σ :
+     σ.(heap) !! l = Some $ Some v →
+     head_step (Store (Val $ LitV $ LitLoc l) (Val w)) σ
+               (Val $ LitV LitUnit) (state_upd_heap <[l:=Some w]> σ)
                []
   | CmpXchgS l v1 v2 vl σ b :
-     σ.(heap) !! l = Some vl →
+     σ.(heap) !! l = Some $ Some vl →
      (* Crucially, this compares the same way as [EqOp]! *)
      vals_compare_safe vl v1 →
      b = bool_decide (vl = v1) →
      head_step (CmpXchg (Val $ LitV $ LitLoc l) (Val v1) (Val v2)) σ
-               (Val $ PairV vl (LitV $ LitBool b)) (if b then state_upd_heap <[l:=v2]> σ else σ)
+               (Val $ PairV vl (LitV $ LitBool b)) (if b then state_upd_heap <[l:=Some v2]> σ else σ)
                []
   | FaaS l i1 i2 σ :
-     σ.(heap) !! l = Some (LitV (LitInt i1)) →
+     σ.(heap) !! l = Some $ Some (LitV (LitInt i1)) →
      head_step (FAA (Val $ LitV $ LitLoc l) (Val $ LitV $ LitInt i2)) σ
-               (Val $ LitV $ LitInt i1) (state_upd_heap <[l:=LitV (LitInt (i1 + i2))]>σ)
+               (Val $ LitV $ LitInt i1) (state_upd_heap <[l:=Some $ LitV (LitInt (i1 + i2))]>σ)
               []
   | ChooseNatS (n:nat) σ:
     head_step ChooseNat σ (Val $ LitV $ LitInt n) σ []
